---
title: "Triangle of Power"
author: "Aj Averett"
date: '2022-07-06'
output:
  html_document: default
  pdf_document: default
  word_document: default
---

```{r setup, include=FALSE}
knitr::opts_chunk$set(echo = TRUE)
```


# The Triangle of Power... $_{a}\stackrel{b}\triangle _{c}$

Below is the equivalents between the triangle of power and standard math notation.
$$
\begin{align*}
& a^b = c & \Leftrightarrow {} \stackrel{b}{_a\triangle_{\phantom{c}}} = c \\
& \sqrt[b]{c} = a & \Leftrightarrow {} \stackrel{}{_a\triangle_{c}} = b\\
& \log_a\left(c\right) = b & \Leftrightarrow {} \stackrel{b}{_\phantom{a}\triangle_{c}} = a
\end{align*}
$$

# Inverse identities

Inverse identities are as follows below: 

e.g. $a = f(f^{-1}(a))$


$$
\begin{align*}
a &= \text{ }
_{\phantom{a}}
\stackrel{b}
\triangle _{    _{a}\stackrel{b}\triangle _{\phantom{c}}    } 
\text{ } &= \text{ }
_{\phantom{a}}
\stackrel{_{a}\stackrel{\phantom{b}}\triangle _{c}}
\triangle _{c} \\\\
b &= \text{ }
_{    _{\phantom{a}}\stackrel{b}\triangle _{c}    }
\stackrel{\phantom{b}}
\triangle _{c} 
\text{ } &= \text{ }
_{a}
\stackrel{\phantom{b}}
\triangle _{    _{a}\stackrel{b}\triangle _{\phantom{c}}    } \\\\ 
c &= \text{ }
_{    _{\phantom{a}}\stackrel{b}\triangle _{c}    }
\stackrel{b}
\triangle _{\phantom{c}} 
\text{ } &= \text{ }
_{a}
\stackrel{    _{a}\stackrel{\phantom{b}}\triangle _{c}    }
\triangle _{\phantom{c}} \\\\
\end{align*}
$$


# Inverse identities

Inverse identities are as follows below: 

$$
\begin{align*}
a &= \sqrt[b]{a^b} &=\sqrt[log_a(c)]{c}
\\\\
b &= \log_a(a^b) &=\log_{\sqrt[a]{c}}(c)
\\\\
c &= (\sqrt[b]{c})^c &=a^{\log_a(c)}
\\\\
\end{align*}
$$


The inverse identities above can be displayed as such in the chart below:

![](top.png)

(yes i made the diagram)

# Properties of these operators

## $a$ remains constant

$$
\begin{align*}
&\text{Properties of Logarithms}
&\text{Properties of Exponents}
\\\\
&
_{a}
\stackrel{\phantom{b}}
\triangle _{xy} 
={}
_{a}\stackrel{\phantom{b}}\triangle _{x} +{}
_{a}\stackrel{\phantom{b}}\triangle _{y}
&
_{a}
\stackrel{x+y}
\triangle _{\phantom{c}} 
={}
_{a}\stackrel{x}\triangle _{\phantom{c}} \times{}
_{a}\stackrel{y}\triangle _{\phantom{c}}
\\\\
&_{a}
\stackrel{\phantom{b}}
\triangle _{\frac{x}{y}} 
={}
_{a}\stackrel{\phantom{b}}\triangle _{x} -{}
_{a}\stackrel{\phantom{b}}\triangle _{y}
&
_{a}
\stackrel{x-y}
\triangle _{\phantom{c}} 
={}
\frac
{_{a}\stackrel{x}\triangle _{\phantom{c}}}
{_{a}\stackrel{y}\triangle _{\phantom{c}}}
\end{align*}
$$

## $b$ remains constant

$$
\begin{align*}
&\text{Properties of Exponents}
&\text{Properties of Roots}
\\\\
&
_{x\times y}
\stackrel{b}
\triangle _{\phantom{c}} 
={}
_{x}\stackrel{b}\triangle _{} \times{}
_{y}\stackrel{b}\triangle _{}
&
_{\phantom{a}}
\stackrel{b}
\triangle _{x\times y} 
={}
_{\phantom{x}}\stackrel{b}\triangle _{x} \times{}
_{\phantom{x}}\stackrel{b}\triangle _{y}
\\\\
&_{\frac{x}{y}}
\stackrel{b}
\triangle _{\phantom{c}} 
={}
\frac
{_{x}\stackrel{b}\triangle _{\phantom{c}} }
{_{y}\stackrel{b}\triangle _{\phantom{c}} }
&
_{\phantom{a}}
\stackrel{b}
\triangle _{\frac{x}{y}} 
=
\frac
{_{\phantom{a}}\stackrel{b}\triangle _{x}}
{_{\phantom{a}}\stackrel{b}\triangle _{y}}
\end{align*}
$$


## $c$ remains constant

$$
\begin{align*}
&\text{Properties of Logarithms}
&\text{Properties of Roots}
\\\\
&
_{x\times y}
\stackrel{\phantom{b}}
\triangle _{c} 
={}
\left(
\left( _{x}\stackrel{}\triangle _{c}\right)^{-1} +{}
\left(_{y}\stackrel{}\triangle _{c}\right)^{-1}
\right)^{-1}
&
_{\phantom{a}}
\stackrel{
  \left(x^{-1}+y^{-1}\right)^{-1}
}
\triangle _{c} 
={}
_{\phantom{x}}\stackrel{x}\triangle _{c} \times{}
_{\phantom{x}}\stackrel{y}\triangle _{c}
\\\\
&
_{\frac{x}{y}}
\stackrel{\phantom{b}}
\triangle _{c} 
={}
\left(
\left( _{x}\stackrel{}\triangle _{c}\right)^{-1} -{}
\left(_{y}\stackrel{}\triangle _{c}\right)^{-1}
\right)^{-1}
&
_{\phantom{a}}
\stackrel{
  \left(x^{-1}-y^{-1}\right)^{-1}
}
\triangle _{c} 
={}
\frac
{_{\phantom{x}}\stackrel{x}\triangle _{c} }
{_{\phantom{x}}\stackrel{y}\triangle _{c}}
\end{align*}
$$


# Properties of these operators (in standard notation)

## $a$ remains constant

$$
\begin{align*}
&\text{Properties of Logarithms}
&\text{Properties of Exponents}
\\\\
&
\log_a(x\times y) = \log_a(x) + \log_b(x)
&
a^{x + y} = a^x \times a ^y
\\\\
&
\log_a(\frac{x}{y}) = \log_a(x) - \log_b(x)
&
a^{x - y} = \frac{a^x}{a^y}
\end{align*}
$$

## $b$ remains constant

$$
\begin{align*}
&\text{Properties of Exponents}
&\text{Properties of Roots}
\\\\
&   xy^b = x^b \times y^b
&   \sqrt[b]{x\times y} = \sqrt[b]{x} \times \sqrt[b]{y}
\\\\
&   \left(\frac{x}{y}\right)^b = \frac{x^b}{y^b}
&   \sqrt[b]{\frac{x}{y}} = \frac{\sqrt[b]{x}}{\sqrt[b]{y}}
\end{align*}
$$

## c remains constant

$$
\begin{align*}
&\text{Properties of Logarithms}
&\text{Properties of Roots}
\\\\
&   \log_{x\times y}(c) = \left(\left(\log_xc\right)^{-1} + \left(\log_yc\right)^{-1}\right)^{-1}
&   \sqrt[(x^{-1}+ y^{-1})^{-1}]{c} = \sqrt[x]{c} \times \sqrt[y]{c}
\\\\
&   \log_{\frac{x}{y}}(c) = \left(\left(\log_xc\right)^{-1} - \left(\log_yc\right)^{-1}\right)^{-1}
&   \sqrt[(x^{-1}- y^{-1})^{-1}]{c} = \frac{\sqrt[x]{c}}{\sqrt[y]{c}}
\end{align*}
$$






$_{a}\stackrel{b}\triangle _{c}$

